<?xml version="1.0" encoding="UTF-8"?>
<!-- Changelog -->
<!-- 30/09/11 (ID) -->
<!-- ROLE ontology meta description removed as it is OWL Lite syntactically incorrect -->
<!-- Added class role:FunctionalityType with property role:realizesWidgetType to reflect WP2 tool categories and their mapping to the widget store widget types -->
<!-- Added property role:relatedFunctio0nality -->
<!-- 07/10/11 (AK, ID) -->
<!-- Added links to glossary -->
<!-- Changed URIs of ToolFunctionality Instances to match WP2 database -->

<rdf:RDF 
	xmlns:dc="http://purl.org/dc/elements/1.1/"
	xmlns:dcterms="http://purl.org/dc/terms/"
	xmlns:owl="http://www.w3.org/2002/07/owl#"
	xmlns:rdf="http://www.w3.org/1999/02/22-rdf-syntax-ns#"
	xmlns:rdfs="http://www.w3.org/2000/01/rdf-schema#"
	xmlns:role="http://purl.org/role/terms/">
	<!-- OWL Lite compatibility tricks -->
	<owl:DatatypeProperty rdf:about="http://purl.org/dc/terms/description"/>
	<owl:DatatypeProperty rdf:about="http://purl.org/dc/terms/title"/>
	<owl:DatatypeProperty rdf:about="http://purl.org/dc/terms/subject"/>
	<owl:ObjectProperty rdf:about="http://purl.org/ontology/cco/core#competence"/>
	<owl:ObjectProperty rdf:about="http://purl.org/ontology/cco/core#habit"/>
	<!-- ROLE ontology meta description down here is "OWL Lite" syntactically incorrect (ID)
		=> we simply comment it in case (or when) OWL Lite compatibility is (will be absolutely) needed.
		 We keep it in the meantime as it's useful for spec file generation (FL)-->
	<owl:Ontology rdf:about="http://purl.org/role/terms/">
		<dcterms:title xml:lang="en">ROLE EU-funded project core ontology</dcterms:title>
		<owl:versionInfo>version 0.1</owl:versionInfo>
		<dcterms:description xml:lang="en">Role Ontology</dcterms:description>
		<rdfs:seeAlso rdf:resource="http://role-project.eu" rdfs:label="ROLE project Homepage"/>
	</owl:Ontology>
	

<!--Redeclaration of classes, need to indicate owl:Class to pass OWL-Lite valid if not explicit dependencies are checked.-->
	<owl:Class rdf:about="http://xmlns.com/foaf/0.1/Agent"/>

<!-- Reusable restrictions that can be subclassed from in various toplevel classes without including a toplevel dummy class, aka Object-->
	<owl:Restriction rdf:nodeID="_dc_title">
	  <owl:onProperty rdf:resource="http://purl.org/dc/terms/title"/>
	  <owl:minCardinality rdf:datatype="http://www.w3.org/2001/XMLSchema#nonNegativeInteger">0</owl:minCardinality>
	</owl:Restriction>

	<owl:Restriction rdf:nodeID="_dc_description">
	  <owl:onProperty rdf:resource="http://purl.org/dc/terms/description"/>
	  <owl:minCardinality rdf:datatype="http://www.w3.org/2001/XMLSchema#nonNegativeInteger">0</owl:minCardinality>
	</owl:Restriction>

	<owl:Restriction rdf:nodeID="_role_icon">
	  <owl:onProperty rdf:resource="http://purl.org/role/terms/iconurl"/>
	  <owl:minCardinality rdf:datatype="http://www.w3.org/2001/XMLSchema#nonNegativeInteger">0</owl:minCardinality>
	</owl:Restriction>


<!-- CLASSES -->
	<owl:Class rdf:about="http://purl.org/role/terms/LearningResource">
		<rdfs:label>Learning Resource</rdfs:label>
		<rdfs:seeAlso rdf:resource="https://ilias.uni-koblenz.de/goto.php?target=git_222_948&amp;client_id=default"/>
		<rdfs:comment>A learning resource is a resource used in a learning context</rdfs:comment>
		<rdfs:subClassOf rdf:nodeID="_dc_description"/>
	</owl:Class>
	<owl:Class rdf:about="http://purl.org/role/terms/Configuration">
		<rdfs:label>Configuration</rdfs:label>
		<rdfs:comment>When a resource is to be added to a context, the resource often need to be contextualized or configured.
		That means providing additional information on this resource that is specific to this context. Making statements
		on the original resource would in the worst case affect other uses of the same resource.
		To reach the resource that is being contextualized/configured use the role:configures property.
		It is up to each subclass to specify if and how properties on the original resource should be 
		copied, provided as a possible override, or always be looked up on the original resource.</rdfs:comment>
	</owl:Class>
	<owl:Class rdf:about="http://purl.org/role/terms/Tool">
		<rdfs:label>Tool</rdfs:label>
		<rdfs:seeAlso rdf:resource="https://ilias.uni-koblenz.de/goto.php?target=git_189_948&amp;client_id=default"/>
		<rdfs:comment>Any software used as a means of accomplishing a learning task or goal.</rdfs:comment>
		<rdfs:subClassOf rdf:nodeID="_dc_description"/>
	</owl:Class>
	<owl:Class rdf:about="http://purl.org/role/terms/ToolConfiguration">
		<rdfs:label>Tool configuration</rdfs:label>
		<rdfs:seeAlso rdf:resource="https://ilias.uni-koblenz.de/goto.php?target=git_215_948&amp;client_id=default"/>
		<rdfs:comment>
		Specification how a tool can be used by providing guidance and a suggested starting configuration for the tool.
		Specifies how a tool can be used by providing guidance and a suggested starting configuration for the tool.
		 An instance of the class Configured Tool should be used to refer to a tool that comes with a set of 
		 configuration information. It is used to describe what is contained in a Bundle in addition
		 to other resources that can be documents, artifacts, or references to users.
		</rdfs:comment>
		<rdfs:subClassOf rdf:resource="http://purl.org/role/terms/Configuration"/>
		<rdfs:subClassOf rdf:resource="http://purl.org/role/terms/Tool"/>
	</owl:Class>
	<owl:Class rdf:about="http://purl.org/role/terms/PersonConfiguration">
		<rdfs:label>Person configuration</rdfs:label>
		<rdfs:seeAlso rdf:resource="https://ilias.uni-koblenz.de/goto.php?target=git_215_948&amp;client_id=default"/>
		<rdfs:comment>Provides information on a person that may directly or at a later point be connected with a foaf:Person.</rdfs:comment>
		<rdfs:subClassOf rdf:resource="http://purl.org/role/terms/Configuration"/>
		<rdfs:subClassOf rdf:resource="http://xmlns.com/foaf/0.1/Person"/>
	</owl:Class>
	<owl:Class rdf:about="http://purl.org/role/terms/Bundle">
		<rdfs:label>Bundle </rdfs:label>
		<rdfs:seeAlso rdf:resource="https://ilias.uni-koblenz.de/goto.php?target=git_219_948&amp;client_id=default"/>
		<rdfs:comment>A bundle is a set of learning resources bundled to fit a particular purpose. 
		Possible resources in a bundle can be documents, widgets, web tools, etc.</rdfs:comment>
	</owl:Class>
	<owl:Class rdf:about="http://purl.org/role/terms/Space">
		<rdfs:label>Space</rdfs:label>
		<rdfs:seeAlso rdf:resource="https://ilias.uni-koblenz.de/goto.php?target=git_193_948&amp;client_id=default"/>
		<rdfs:comment>A space is a setting where a group of users can perform one or several activities.</rdfs:comment>
		<rdfs:subClassOf rdf:resource="http://purl.org/role/terms/Bundle"/>
		<rdfs:subClassOf rdf:resource="http://purl.org/role/terms/Configuration"/>
		<rdfs:subClassOf rdf:resource="http://rdfs.org/sioc/ns#Site"/>
		<rdfs:subClassOf rdf:resource="http://xmlns.com/foaf/0.1/Group"/>
	</owl:Class>

	<owl:Class rdf:about="http://purl.org/role/terms/Widget">
		<rdfs:label>Widget</rdfs:label>
		<rdfs:seeAlso rdf:resource="https://ilias.uni-koblenz.de/goto.php?target=git_191_948&amp;client_id=default"/>
		<rdfs:comment>Widgets are small tools that provide functionality in a user interface.Widgets
		 follow some standard that makes it possible to run it in different environments.A widget can
		  refer to at least one functionality. Widgets are often Web-enabled. </rdfs:comment>
		<rdfs:subClassOf rdf:resource="http://purl.org/role/terms/Tool"/>
	</owl:Class>
	

	<owl:Class rdf:about="http://purl.org/role/terms/OpenSocialGadget">
		<rdfs:label>Open Social Gadget</rdfs:label>
		<rdfs:seeAlso rdf:resource="https://ilias.uni-koblenz.de/goto.php?target=git_191_948&amp;client_id=default"/>
		<rdfs:comment>OpenSocial standard provide a specification for widgets that are called "applications"
		 or "gadgets". Tools following complient to this standard should be typed with role:OpenSocialGadget 
		 a subclass of role:Widget </rdfs:comment>
		<rdfs:subClassOf rdf:resource="http://purl.org/role/terms/Widget"/>
	</owl:Class>
	<owl:Class rdf:about="http://purl.org/role/terms/W3CWidget">
		<rdfs:label>W3C Widget</rdfs:label>
		<rdfs:comment>W3C Widgets are full-fledged client-side applications that are authored using Web standards 
		such as HTML and packaged for distribution. They are typically downloaded and installed on a client machine 
		or device where they run as stand-alone applications, but they can also be embedded into Web pages and run in 
		a Web browser. Examples range from simple clocks, stock tickers, news casters, games and weather forecasters, 
		to complex applications that pull data from multiple sources to be "mashed-up" and presented to a user in 
		some interesting and useful way.</rdfs:comment>
		<rdfs:subClassOf rdf:resource="http://purl.org/role/terms/Widget"/>
	</owl:Class>
	
	<owl:Class rdf:about="http://purl.org/role/terms/Category">
		<rdfs:label>Category</rdfs:label>
		<rdfs:comment>Class used to describe the category of a Tool. Used with the property role:category from Tool. 
		Functionalities may reference categories directly but then via the role:providedByCategory property.</rdfs:comment>
	</owl:Class>

<!--#####     PROPERTIES    ####  -->

	<owl:ObjectProperty rdf:about="http://purl.org/role/terms/owner">
		<rdfs:label>owner</rdfs:label>
		<rdfs:comment>The owner of the space, may be repeated to indicate multiple owners.</rdfs:comment>
		<rdfs:domain rdf:resource="http://purl.org/role/terms/Space"/>
		<rdfs:range rdf:resource="http://purl.org/role/terms/PersonConfiguration"/>
	</owl:ObjectProperty>

	<owl:ObjectProperty rdf:about="http://purl.org/role/terms/member">
		<rdfs:label>member</rdfs:label>
		<rdfs:comment>Indicates the members of a space.</rdfs:comment>
		<rdfs:domain rdf:resource="http://purl.org/role/terms/Space"/>
		<rdfs:range rdf:resource="http://purl.org/role/terms/PersonConfiguration"/>
		<rdfs:subPropertyOf rdf:resource="http://xmlns.com/foaf/0.1/member"/>
	</owl:ObjectProperty>

	<owl:ObjectProperty rdf:about="http://purl.org/role/terms/category">
		<rdfs:label>category</rdfs:label>
		<rdfs:comment>property used to describe the category of a Tool. Points to an instance of the class role:Category.</rdfs:comment>
		<rdfs:domain rdf:resource="http://purl.org/role/terms/Tool"/>
		<rdfs:range rdf:resource="http://purl.org/role/terms/Category"/>
	</owl:ObjectProperty>

	<owl:ObjectProperty rdf:about="http://purl.org/role/terms/providedByCategory">
		<rdfs:label>provided by category</rdfs:label>
		<rdfs:comment>Property is used to describe that the functionality is often provided by tools found in the given category.</rdfs:comment>
		<rdfs:domain rdf:resource="http://purl.org/role/terms/Functionality"/>
		<rdfs:range rdf:resource="http://purl.org/role/terms/Category"/>
	</owl:ObjectProperty>

	<owl:ObjectProperty rdf:about="http://purl.org/role/terms/providedBy">
		<rdfs:label>provided by</rdfs:label>
		<rdfs:comment>Points from a Functionality to a Tool that provides this functionality.</rdfs:comment>
		<rdfs:domain rdf:resource="http://purl.org/role/terms/Functionality"/>
		<rdfs:range rdf:resource="http://purl.org/role/terms/Tool"/>
	</owl:ObjectProperty>
	<owl:ObjectProperty rdf:about="http://purl.org/role/terms/provides">
		<rdfs:label>provides</rdfs:label>
		<rdfs:comment>Points from a Tool to a Functionality offered by this tool.</rdfs:comment>
		<rdf:type rdf:resource="http://www.w3.org/2002/07/owl#InverseFunctionalProperty"/>
		<owl:inverseOf rdf:resource="http://purl.org/role/terms/providedBy"/>
		<rdfs:domain rdf:resource="http://purl.org/role/terms/Tool"/>
		<rdfs:range rdf:resource="http://purl.org/role/terms/Functionality"/>
	</owl:ObjectProperty>
	<owl:ObjectProperty rdf:about="http://purl.org/role/terms/data">
		<rdfs:label>data</rdfs:label>
		<rdfs:comment>Property linking a bundle to one or several resources containing data relevant for the bundle.</rdfs:comment>
		<rdfs:domain rdf:resource="http://purl.org/role/terms/Bundle"/>
		<rdfs:range rdf:resource="http://www.w3.org/2002/07/owl#Thing"/>
	</owl:ObjectProperty>
	<owl:ObjectProperty rdf:about="http://purl.org/role/terms/tool">
		<rdfs:label>tool</rdfs:label>
		<rdfs:comment>Connects a ToolConfiguration to a Bundle.</rdfs:comment>
		<rdfs:domain rdf:resource="http://purl.org/role/terms/Bundle"/>
		<rdfs:range rdf:resource="http://purl.org/role/terms/ToolConfiguration"/>
	</owl:ObjectProperty>
	<owl:ObjectProperty rdf:about="http://purl.org/role/terms/configures">
		<rdfs:label>configures</rdfs:label>
		<rdfs:comment>Points to which resource the Configuration provides contextualized information for.</rdfs:comment>
		<rdfs:domain rdf:resource="http://purl.org/role/terms/Configuration"/>
		<rdfs:range rdf:resource="http://www.w3.org/2002/07/owl#Thing"/>
	</owl:ObjectProperty>
	<owl:ObjectProperty rdf:about="http://purl.org/role/terms/overlay">
		<rdfs:label>overlay</rdfs:label>
		<rdfs:comment>Overlays a Configuration with another Configuration.
		For example when the owner of a space has provided a ToolConfiguration with default settings for a tool,
		one of the members can provide an additional Configuration that overrides those settings, 
		these settings will only be visible for that member.</rdfs:comment>
		<rdfs:domain rdf:resource="http://purl.org/role/terms/Configuration"/>
		<rdfs:range rdf:resource="http://purl.org/role/terms/Configuration"/>
	</owl:ObjectProperty>
	<owl:DatatypeProperty rdf:about="http://purl.org/role/terms/userPreferences">
		<rdfs:label>user Preferences</rdfs:label>
		<rdfs:comment>for a ConfiguredTool instance, gives the XML description of the user's preferences for the corresponding tool.</rdfs:comment>
		<rdfs:domain rdf:resource="http://purl.org/role/terms/ToolConfiguration"/>
		<rdfs:range rdf:resource="http://www.w3.org/2001/XMLSchema#string"/>
	</owl:DatatypeProperty>


	<!-- ** COMPETENCE part of the ontology, ver2 **-->
	<owl:Class rdf:about="http://purl.org/role/terms/Competence">
		<rdfs:label>Competence</rdfs:label>
		<rdfs:comment>A generic competence</rdfs:comment>
		<rdfs:subClassOf rdf:nodeID="_dc_description"/>
		<rdfs:subClassOf rdf:nodeID="_dc_title"/>
	</owl:Class>

	<owl:Class rdf:about="http://purl.org/role/terms/Level">
		<rdfs:label>Competence level</rdfs:label>
		<rdfs:comment>Subclasses gives a more precise semantics of the kind of level.</rdfs:comment>
		<rdfs:subClassOf rdf:nodeID="_dc_description"/>
		<rdfs:subClassOf rdf:nodeID="_dc_title"/>
	</owl:Class>

	<owl:Class rdf:about="http://purl.org/role/terms/EQF">
		<rdfs:label>EQF level</rdfs:label>
		<rdfs:comment>European Qualification Framework (EQF) provides seven levels ranging from beginner to expert.</rdfs:comment>
		<rdfs:subClassOf rdf:resource="http://purl.org/role/terms/Level"/>
	</owl:Class>

	<owl:Class rdf:about="http://purl.org/role/terms/ToolCompetence">
		<rdfs:label>Tool competence</rdfs:label>
		<rdfs:comment>Correspond to the competence of using a certain kind of tool with a specific technique, i.e. points to one or several Functionalitites and a single Technique.</rdfs:comment>
		<rdfs:subClassOf rdf:resource="http://purl.org/role/terms/Competence"/>
		<owl:subClassOf>
		  <owl:Restriction>
		    <owl:onProperty rdf:resource="http://purl.org/role/terms/topic"/>
		    <owl:allValuesFrom rdf:resource="http://purl.org/role/terms/Functionality"/>
		  </owl:Restriction>
		</owl:subClassOf>
	</owl:Class>
	
	<owl:Class rdf:about="http://purl.org/role/terms/SRLCompetence">
		<rdfs:label>SRL competence</rdfs:label>
		<rdfs:comment>Correspond to the Self-Regulated Learning (SRL) competence, points to a SRLStrategy and possibly a EQFLevel.</rdfs:comment>
		<rdfs:subClassOf rdf:resource="http://purl.org/role/terms/Competence"/>
		<owl:subClassOf>
		  <owl:Restriction>
		    <owl:onProperty rdf:resource="http://purl.org/role/terms/topic"/>
		    <owl:allValuesFrom rdf:resource="http://purl.org/role/terms/SRLStrategy"/>
		  </owl:Restriction>
		</owl:subClassOf>
	</owl:Class>

	<owl:Class rdf:about="http://purl.org/role/terms/DomainCompetence">
		<rdfs:label>Domain competence</rdfs:label>
		<rdfs:comment>Correspond to the competence within a specific domain.</rdfs:comment>
		<rdfs:subClassOf rdf:resource="http://purl.org/role/terms/Competence"/>
		<owl:subClassOf>
		  <owl:Restriction>
		    <owl:onProperty rdf:resource="http://purl.org/role/terms/proficiencyLevel"/>
		    <owl:allValuesFrom rdf:resource="http://purl.org/role/terms/EQF"/>
		  </owl:Restriction>
		</owl:subClassOf>
	</owl:Class>

	<owl:ObjectProperty rdf:about="http://purl.org/role/terms/topic">
		<rdfs:label>Topic</rdfs:label>
		<rdfs:comment>Property should be used to clarify the topic of a comptence.</rdfs:comment>
		<rdfs:domain rdf:resource="http://purl.org/role/terms/Competence"/>
		<rdfs:range rdf:resource="http://www.w3.org/2002/07/owl#Thing"/>
	</owl:ObjectProperty>

	<owl:ObjectProperty rdf:about="http://purl.org/role/terms/technique">
		<rdfs:label>Technique</rdfs:label>
		<rdfs:comment>Property should be used to clarify the learning technique the ToolComptence referres to.</rdfs:comment>
		<rdfs:domain rdf:resource="http://purl.org/role/terms/ToolCompetence"/>
		<rdfs:range rdf:resource="http://purl.org/role/terms/LearningTechnique"/>
	</owl:ObjectProperty>

	<owl:ObjectProperty rdf:about="http://purl.org/role/terms/proficiencyLevel">
		<rdfs:label>Proficiency level</rdfs:label>
		<rdfs:comment>Property should be used to indicate the proficiency level a user reached with respect to the topic of this competence.</rdfs:comment>
		<rdfs:domain rdf:resource="http://purl.org/role/terms/Competence"/>
		<rdfs:range rdf:resource="http://purl.org/role/terms/Level"/>
	</owl:ObjectProperty>
	
	<owl:Class rdf:about="http://purl.org/role/terms/SRLStrategy">
	  <rdfs:label>SRL strategy</rdfs:label>
	  <rdfs:subClassOf rdf:resource="http://purl.org/role/terms/LearningStrategy"/>
	  <rdfs:seeAlso rdf:resource="https://ilias.uni-koblenz.de/goto.php?target=git_240_948&amp;client_id=default"/>
	  <rdfs:comment>An SRL Strategy is a strategy that is applied for self-regulated learning.</rdfs:comment>
	</owl:Class>

	<owl:Class rdf:about="http://purl.org/role/terms/CognitiveStrategy">
	  <rdfs:label>Cognitive strategy</rdfs:label>
	  <rdfs:subClassOf rdf:resource="http://purl.org/role/terms/SRLStrategy"/>
	  <rdfs:seeAlso rdf:resource="https://ilias.uni-koblenz.de/goto.php?target=git_237_948&amp;client_id=default"/>
	  <rdfs:comment>A cognitive strategy is a strategy which enables a learner to encode new material and facilitate the organization and retrieval of information.</rdfs:comment>
	</owl:Class>

	<owl:Class rdf:about="http://purl.org/role/terms/MetacognitiveStrategy">
	  <rdfs:label>Metacognitive strategy</rdfs:label>
	  <rdfs:subClassOf rdf:resource="http://purl.org/role/terms/SRLStrategy"/>
	  <rdfs:seeAlso rdf:resource="https://ilias.uni-koblenz.de/goto.php?target=git_238_948&amp;client_id=default"/>
	  <rdfs:comment>A meta-cognitive strategy is a strategy which enables a learner to control the own learning process.</rdfs:comment>
	</owl:Class>	

	<owl:Class rdf:about="http://purl.org/role/terms/ResourceManagementStrategy">
	  <rdfs:label>ResourceManagementStrategy</rdfs:label>
	  <rdfs:subClassOf rdf:resource="http://purl.org/role/terms/SRLStrategy"/>
	  <rdfs:seeAlso rdf:resource="https://ilias.uni-koblenz.de/goto.php?target=git_239_948&amp;client_id=default"/>
	  <rdfs:comment>A resource management strategy is a strategy which enables a learner to control and organize available resources including learning material, people, time and other.</rdfs:comment>
	</owl:Class>	
	
	<owl:ObjectProperty rdf:about="http://purl.org/role/terms/aquiredCompetence">
		<rdfs:label>Aquired competence</rdfs:label>
		<rdfs:comment>Property used to link a user (foaf profile) with a competence he or she has AQUIRED.
			In ROLE terminology, it can also be refered to as the competence profile of a learner.</rdfs:comment>
		<rdfs:seeAlso rdf:resource="https://ilias.uni-koblenz.de/goto.php?target=git_96_948&amp;client_id=default" />
	</owl:ObjectProperty>
	
	<owl:ObjectProperty rdf:about="http://purl.org/role/terms/goalCompetence">
		<rdfs:label>Goal competence</rdfs:label>
		<rdfs:comment>Property used to link a user (foaf profile) with a GOAL competence, i.e. a competence
		 he/she PLANS ON AQUIRING.</rdfs:comment>
		<rdfs:seeAlso rdf:resource="https://ilias.uni-koblenz.de/goto.php?target=git_167_948&amp;client_id=default" />
		<rdfs:subPropertyOf rdf:resource="http://purl.org/ontology/cco/core#habit"/>
	</owl:ObjectProperty>
	

	<!--######  Learning ontology-->
	<owl:Class rdf:about="http://purl.org/role/terms/LearningActivity">
	  <rdfs:label>Learning activity</rdfs:label>
	  <rdfs:subClassOf rdf:nodeID="_dc_title"/>
	  <rdfs:subClassOf rdf:nodeID="_dc_description"/>
	  <rdfs:subClassOf rdf:nodeID="_role_icon"/>
	  <rdfs:comment>A learning activity is a representation of a necessary operation to be performed to complete a learning task. It consists of decision activities (DA) or concrete activities (CA). </rdfs:comment>
	  <rdfs:seeAlso rdf:resource="https://ilias.uni-koblenz.de/goto.php?target=git_139_948&amp;client_id=default"/>
	</owl:Class>
	<owl:Class rdf:about="http://purl.org/role/terms/ConcreteActivity">
	  <rdfs:label>Concrete activity</rdfs:label>
	  <owl:disjointWith rdf:resource="http://purl.org/role/terms/DecisionActivity"/>
	  <rdfs:subClassOf rdf:resource="http://purl.org/role/terms/LearningActivity"/>
	  <rdfs:comment>A concrete activity is a step in the learning process. </rdfs:comment>
	  <rdfs:seeAlso rdf:resource="https://ilias.uni-koblenz.de/goto.php?target=git_216_948&amp;client_id=default"/>
	</owl:Class>
	<owl:Class rdf:about="http://purl.org/role/terms/DecisionActivity">
	  <rdfs:label>Decision activity</rdfs:label>
	  <owl:disjointWith rdf:resource="http://purl.org/role/terms/ConcreteActivity"/>
	  <rdfs:subClassOf rdf:resource="http://purl.org/role/terms/LearningActivity"/>
	  <rdfs:seeAlso rdf:resource="https://ilias.uni-koblenz.de/goto.php?target=git_234_948&amp;client_id=default"/>
	  <rdfs:comment>A decision activity is a selection of references to at least one learning strategy.</rdfs:comment>
	</owl:Class>
	<owl:Class rdf:about="http://purl.org/role/terms/LearningStrategy">
	  <rdfs:label>Learning strategy</rdfs:label>
	  <rdfs:subClassOf rdf:nodeID="_dc_title"/>
	  <rdfs:subClassOf rdf:nodeID="_dc_description"/>
	  <rdfs:subClassOf rdf:nodeID="_role_icon"/>
	  <rdfs:seeAlso rdf:resource="https://ilias.uni-koblenz.de/goto.php?target=git_177_948&amp;client_id=default"/>
	  <rdfs:comment>A learning strategy is a sequence of learning activities (concrete activities and decision activities).</rdfs:comment>
	</owl:Class>
	<owl:Class rdf:about="http://purl.org/role/terms/LearningTechnique">
	  <rdfs:label>Learning technique</rdfs:label>
	  <rdfs:subClassOf rdf:resource="http://purl.org/role/terms/LearningStrategy"/>
	  <owl:equivalentClass>
	    <owl:Restriction>
	      <owl:onProperty rdf:resource="http://purl.org/role/terms/activity"/>
	      <owl:allValuesFrom rdf:resource="http://purl.org/role/terms/ConcreteActivity"/>
	    </owl:Restriction>
	  </owl:equivalentClass>
	  <rdfs:seeAlso rdf:resource="https://ilias.uni-koblenz.de/goto.php?target=git_178_948&amp;client_id=default"/>
	  <rdfs:comment>A learning technique is a exceptional case of learning strategy consisting only of concrete activities.</rdfs:comment>
	</owl:Class>
	<owl:Class rdf:about="http://purl.org/role/terms/Functionality">
	  <rdfs:label>Functionality</rdfs:label>
	  <rdfs:subClassOf rdf:nodeID="_dc_title"/>
	  <rdfs:subClassOf rdf:nodeID="_dc_description"/>
	  <rdfs:subClassOf rdf:nodeID="_role_icon"/>
	  <rdfs:seeAlso rdf:resource="https://ilias.uni-koblenz.de/goto.php?target=git_214_948&amp;client_id=default"/>
	  <rdfs:comment>Functionality describes the purpose of a tool or service for which it is designed and its capability to fulfill specific functions.</rdfs:comment>
	</owl:Class>

	<!-- PROPERTIES -->
	<owl:ObjectProperty rdf:about="http://purl.org/role/terms/supportedBy">
	  <rdfs:label>supported by</rdfs:label>
	  <rdfs:comment>Points to a Functionality that the Learning activity/Learning technique is supported by.</rdfs:comment>
	  <rdfs:domain>
	    <owl:Class>
	      <owl:unionOf rdf:parseType="Collection">
		<rdf:Description rdf:about="http://purl.org/role/terms/LearningActivity"/>
		<rdf:Description rdf:about="http://purl.org/role/terms/LearningTechnique"/>
	      </owl:unionOf>
	    </owl:Class>
	  </rdfs:domain>
	  <rdfs:range rdf:resource="http://purl.org/role/terms/Functionality"/>
	</owl:ObjectProperty>

	<owl:ObjectProperty rdf:about="http://purl.org/role/terms/requiresCompletionOf">
	  <rdfs:label>requires completion of</rdfs:label>
	  <rdfs:comment>Points to another learning activity that must have been completed before starting the current learning activity.</rdfs:comment>
	  <rdf:type rdf:resource="http://www.w3.org/2002/07/owl#TransitiveProperty"/>
	  <rdfs:domain rdf:resource="http://purl.org/role/terms/LearningActivity"/>
	  <rdfs:range rdf:resource="http://purl.org/role/terms/LearningActivity"/>
	</owl:ObjectProperty>

	<owl:ObjectProperty rdf:about="http://purl.org/role/terms/option">
	  <rdfs:label>option</rdfs:label>
	  <rdfs:comment>Points to one or several learning strategies that the user should choose among.</rdfs:comment>
	  <rdfs:domain rdf:resource="http://purl.org/role/terms/DecisionActivity"/>
	  <rdfs:range rdf:resource="http://purl.org/role/terms/LearningStrategy"/>
	</owl:ObjectProperty>

	<owl:ObjectProperty rdf:about="http://purl.org/role/terms/activity">
	  <rdfs:label>activity</rdfs:label>
	  <rdfs:comment>A learning activity that is part of this learning strategy.</rdfs:comment>
	  <rdfs:domain rdf:resource="http://purl.org/role/terms/LearningStrategy"/>
	  <rdfs:range rdf:resource="http://purl.org/role/terms/LearningActivity"/>
	</owl:ObjectProperty>

	<owl:ObjectProperty rdf:about="http://purl.org/role/terms/icon">
	  <rdfs:label>icon</rdfs:label>
	  <rdfs:comment>Specifies an image that is to be used as icon for the resource.</rdfs:comment>
	  <rdfs:domain rdf:resource="http://www.w3.org/2000/01/rdf-schema#Resource"/>
	  <rdfs:range rdf:resource="http://xmlns.com/foaf/0.1/Image"/>
	</owl:ObjectProperty>
</rdf:RDF>