<?xml version="1.0" encoding="UTF-8"?>
<!-- Change Log -->
<!-- 07/10/11(AK)  -->
<!-- Added links to glossary -->
<rdf:RDF xmlns:dcterms="http://purl.org/dc/terms"
	 xmlns:owl="http://www.w3.org/2002/07/owl#"
	 xmlns:rdf="http://www.w3.org/1999/02/22-rdf-syntax-ns#"
	 xmlns:rdfs="http://www.w3.org/2000/01/rdf-schema#"
	 xmlns:role="http://purl.org/role/terms/">

	<!-- OWL Lite compatibility tricks -->
	<owl:DatatypeProperty rdf:about="http://purl.org/dc/terms/description"/>
	<owl:DatatypeProperty rdf:about="http://purl.org/dc/terms/title"/>


	<owl:Class rdf:about="http://purl.org/role/terms/LearningActivity">
	  <rdfs:label>Learning activity</rdfs:label>
	  <rdfs:subClassOf rdf:nodeID="_dc_title"/>
	  <rdfs:subClassOf rdf:nodeID="_dc_description"/>
	  <rdfs:subClassOf rdf:nodeID="_role_icon"/>
	  <rdfs:comment>A learning activity is a representation of a necessary operation to be performed to complete a learning task. It consists of decision activities (DA) or concrete activities (CA). </rdfs:comment>
	  <rdfs:seeAlso rdf:resource="https://ilias.uni-koblenz.de/goto.php?target=git_139_948&amp;client_id=default"/>
	</owl:Class>
	<owl:Class rdf:about="http://purl.org/role/terms/ConcreteActivity">
	  <rdfs:label>Concrete activity</rdfs:label>
	  <owl:disjointWith rdf:resource="http://purl.org/role/terms/DecisionActivity"/>
	  <rdfs:subClassOf rdf:resource="http://purl.org/role/terms/LearningActivity"/>
	  <rdfs:comment>A concrete activity is a step in the learning process. </rdfs:comment>
	  <rdfs:seeAlso rdf:resource="https://ilias.uni-koblenz.de/goto.php?target=git_216_948&amp;client_id=default"/>
	</owl:Class>
	<owl:Class rdf:about="http://purl.org/role/terms/DecisionActivity">
	  <rdfs:label>Decision activity</rdfs:label>
	  <owl:disjointWith rdf:resource="http://purl.org/role/terms/ConcreteActivity"/>
	  <rdfs:subClassOf rdf:resource="http://purl.org/role/terms/LearningActivity"/>
	  <rdfs:seeAlso rdf:resource="https://ilias.uni-koblenz.de/goto.php?target=git_234_948&amp;client_id=default"/>
	  <rdfs:comment>A decision activity is a selection of references to at least one learning strategy.</rdfs:comment>
	</owl:Class>
	<owl:Class rdf:about="http://purl.org/role/terms/LearningStrategy">
	  <rdfs:label>Learning strategy</rdfs:label>
	  <rdfs:subClassOf rdf:nodeID="_dc_title"/>
	  <rdfs:subClassOf rdf:nodeID="_dc_description"/>
	  <rdfs:subClassOf rdf:nodeID="_role_icon"/>
	  <rdfs:seeAlso rdf:resource="https://ilias.uni-koblenz.de/goto.php?target=git_177_948&amp;client_id=default"/>
	  <rdfs:comment>A learning strategy is a sequence of learning activities (concrete activities and decision activities).</rdfs:comment>
	</owl:Class>
	<owl:Class rdf:about="http://purl.org/role/terms/LearningTechnique">
	  <rdfs:label>Learning technique</rdfs:label>
	  <rdfs:subClassOf rdf:resource="http://purl.org/role/terms/LearningStrategy"/>
	  <owl:equivalentClass>
	    <owl:Restriction>
	      <owl:onProperty rdf:resource="http://purl.org/role/terms/activity"/>
	      <owl:allValuesFrom rdf:resource="http://purl.org/role/terms/ConcreteActivity"/>
	    </owl:Restriction>
	  </owl:equivalentClass>
	  <rdfs:seeAlso rdf:resource="https://ilias.uni-koblenz.de/goto.php?target=git_178_948&amp;client_id=default"/>
	  <rdfs:comment>A learning technique is a exceptional case of learning strategy consisting only of concrete activities.</rdfs:comment>
	</owl:Class>
	<owl:Class rdf:about="http://purl.org/role/terms/Functionality">
	  <rdfs:label>Functionality</rdfs:label>
	  <rdfs:subClassOf rdf:nodeID="_dc_title"/>
	  <rdfs:subClassOf rdf:nodeID="_dc_description"/>
	  <rdfs:subClassOf rdf:nodeID="_role_icon"/>
	  <rdfs:seeAlso rdf:resource="https://ilias.uni-koblenz.de/goto.php?target=git_214_948&amp;client_id=default"/>
	  <rdfs:comment>Functionality describes the purpose of a tool or service for which it is designed and its capability to fulfill specific functions.</rdfs:comment>
	</owl:Class>

	<!-- PROPERTIES -->
	<owl:ObjectProperty rdf:about="http://purl.org/role/terms/supportedBy">
	  <rdfs:label>supported by</rdfs:label>
	  <rdfs:comment>Points to a Functionality that the Learning activity/Learning technique is supported by.</rdfs:comment>
	  <rdfs:domain>
	    <owl:Class>
	      <owl:unionOf rdf:parseType="Collection">
		<rdf:Description rdf:about="http://purl.org/role/terms/LearningActivity"/>
		<rdf:Description rdf:about="http://purl.org/role/terms/LearningTechnique"/>
	      </owl:unionOf>
	    </owl:Class>
	  </rdfs:domain>
	  <rdfs:range rdf:resource="http://purl.org/role/terms/Functionality"/>
	</owl:ObjectProperty>

	<owl:ObjectProperty rdf:about="http://purl.org/role/terms/requiresCompletionOf">
	  <rdfs:label>requires completion of</rdfs:label>
	  <rdfs:comment>Points to another learning activity that must have been completed before starting the current learning activity.</rdfs:comment>
	  <rdf:type rdf:resource="http://www.w3.org/2002/07/owl#TransitiveProperty"/>
	  <rdfs:domain rdf:resource="http://purl.org/role/terms/LearningActivity"/>
	  <rdfs:range rdf:resource="http://purl.org/role/terms/LearningActivity"/>
	</owl:ObjectProperty>

	<owl:ObjectProperty rdf:about="http://purl.org/role/terms/option">
	  <rdfs:label>option</rdfs:label>
	  <rdfs:comment>Points to one or several learning strategies that the user should choose among.</rdfs:comment>
	  <rdfs:domain rdf:resource="http://purl.org/role/terms/DecisionActivity"/>
	  <rdfs:range rdf:resource="http://purl.org/role/terms/LearningStrategy"/>
	</owl:ObjectProperty>

	<owl:ObjectProperty rdf:about="http://purl.org/role/terms/activity">
	  <rdfs:label>activity</rdfs:label>
	  <rdfs:comment>A learning activity that is part of this learning strategy.</rdfs:comment>
	  <rdfs:domain rdf:resource="http://purl.org/role/terms/LearningStrategy"/>
	  <rdfs:range rdf:resource="http://purl.org/role/terms/LearningActivity"/>
	</owl:ObjectProperty>

	<owl:ObjectProperty rdf:about="http://purl.org/role/terms/icon">
	  <rdfs:label>icon</rdfs:label>
	  <rdfs:comment>Specifies an image that is to be used as icon for the resource.</rdfs:comment>
	  <rdfs:domain rdf:resource="http://www.w3.org/2000/01/rdf-schema#Resource"/>
	  <rdfs:range rdf:resource="http://xmlns.com/foaf/0.1/Image"/>
	</owl:ObjectProperty>

	<!-- Reusable restrictions that can be subclassed from in various toplevel classes without including a toplevel dummy class, aka Object-->
	<owl:Restriction rdf:nodeID="_dc_title">
	  <owl:onProperty rdf:resource="http://purl.org/dc/terms/title"/>
	  <owl:minCardinality rdf:datatype="http://www.w3.org/2001/XMLSchema#nonNegativeInteger">0</owl:minCardinality>
	</owl:Restriction>

	<owl:Restriction rdf:nodeID="_dc_description">
	  <owl:onProperty rdf:resource="http://purl.org/dc/terms/description"/>
	  <owl:minCardinality rdf:datatype="http://www.w3.org/2001/XMLSchema#nonNegativeInteger">0</owl:minCardinality>
	</owl:Restriction>

	<owl:Restriction rdf:nodeID="_role_icon">
	  <owl:onProperty rdf:resource="http://purl.org/role/terms/iconurl"/>
	  <owl:minCardinality rdf:datatype="http://www.w3.org/2001/XMLSchema#nonNegativeInteger">0</owl:minCardinality>
	</owl:Restriction>
</rdf:RDF>
